fix lints

Batteries/Data/Iterators/Scan.lean
@@ -14,25 +14,26 @@ namespace Std.Iterators
 /--
   Internal state for the ScanM combinator
 -/
-structure ScanM (α : Type w) (m : Type w → Type w') (n : Type w → Type w'') (β : Type w)
-    (γ : Type w) (f : γ → β → n γ) where
+structure ScanM (α : Type w) (m : Type w → Type w') (n : Type w → Type w'')
+    (β : Type w) (γ : Type w) (f : γ → β → n γ) where
   /-- Inner iterator -/
   inner : α
   /-- Current accumulated value -/
   acc : γ
-  /-- Whether we have emitted the initial value (and therefore should begin yielding from the iterator) -/
+  /-- Whether we have emitted the initial value
+    (and therefore should begin yielding from the iterator) -/
   emittedInit : Bool
 
 namespace ScanM
 
 variable {α β γ : Type w} {m : Type w → Type w'} {n : Type w → Type w''}
-    {f : γ → β → n γ} [Iterator α m β]
+  {f : γ → β → n γ} [Iterator α m β]
 /--
-`it.IsPlausibleStep` is the proposition that `step` is a possible next step from the `scanM` iterator `it`.
-This is mostly an internal implementation detail used to prove termination.
+`it.IsPlausibleStep` is the proposition that `step` is a possible next step from the `scanM`
+iterator `it`. This is mostly an internal implementation detail used to prove termination.
 -/
-inductive IsPlausibleStep (it : @IterM (ScanM α m n β γ f) n γ)
-    : IterStep (@IterM (ScanM α m n β γ f) n γ) γ → Prop where
+inductive IsPlausibleStep (it : @IterM (ScanM α m n β γ f) n γ) :
+    IterStep (@IterM (ScanM α m n β γ f) n γ) γ → Prop where
 
   /-- If we haven't emitted anything yet (emittedInit is false),
       we set it to true and do not update the internal iterator state
@@ -65,7 +66,6 @@ inductive IsPlausibleStep (it : @IterM (ScanM α m n β γ f) n γ)
       Iterator.IsPlausibleStep (⟨it.internalState.inner⟩ : IterM m β) .done →
       IsPlausibleStep it .done
 
-
 instance instIterator [Monad n] [MonadLiftT m n] :
     Iterator (ScanM α m n β γ f) n γ where
 
@@ -96,7 +96,7 @@ instance [Monad n] [MonadLiftT m n] :
     IteratorLoop (ScanM α m n β γ f) n n :=
   .defaultImplementation
 
-instance {o : Type w → Type x} [Monad n] [MonadLiftT m n] [Monad o] [MonadLiftT n o] :
+instance {o : Type w → Type x} [Monad n] [MonadLiftT m n] [Monad o] :
     IteratorCollect (ScanM α m n β γ f) n o :=
   .defaultImplementation
 
@@ -105,7 +105,7 @@ private def finRel (scanIt' scanIt : @IterM (ScanM α m n β γ f) n γ) : Prop 
   match scanIt.internalState.emittedInit, scanIt'.internalState.emittedInit with
   | false, true => True
   | true, true => (⟨scanIt'.internalState.inner⟩ : IterM m β).IsPlausibleSuccessorOf
-                    ⟨scanIt.internalState.inner⟩
+      ⟨scanIt.internalState.inner⟩
   | _, _ => False
 
 private theorem acc_finRel_emittedTrue [Finite α m (β := β)]
@@ -132,15 +132,13 @@ private theorem acc_finRel_emittedFalse [Finite α m (β := β)]
     -- this leads to a contradiction
     . simp_all [finRel]
 
-
-private theorem acc_finRel [Finite α m (β := β)] (scanIt : @IterM (ScanM α m n β γ f) n γ)
-    : Acc finRel scanIt :=
+private theorem acc_finRel [Finite α m (β := β)] (scanIt : @IterM (ScanM α m n β γ f) n γ) :
+    Acc finRel scanIt :=
   if h : scanIt.internalState.emittedInit
     then acc_finRel_emittedTrue _ ‹_›
     else acc_finRel_emittedFalse _ (by simp only [h])
 
-
-private instance instFinRel [Monad m] [Monad n] [MonadLiftT m n] [Finite α m (β := β)] :
+private def instFinRel [Monad m] [Monad n] [MonadLiftT m n] [Finite α m (β := β)] :
     FinitenessRelation (ScanM α m n β γ f) n where
   rel := finRel
   wf := ⟨acc_finRel⟩
@@ -153,24 +151,21 @@ private instance instFinRel [Monad m] [Monad n] [MonadLiftT m n] [Finite α m (�
     . exact IterM.isPlausibleSuccessorOf_of_yield ‹_›
     . exact IterM.isPlausibleSuccessorOf_of_skip  ‹_›
 
-instance [Finite α m (β := β)] [Monad m] [Monad n] [MonadLiftT m n]
-    : Finite (ScanM α m n β γ f) n :=
+instance [Finite α m (β := β)] [Monad m] [Monad n] [MonadLiftT m n] :
+    Finite (ScanM α m n β γ f) n :=
   .of_finitenessRelation instFinRel
-
 
 /-- Productiveness relation for ScanM -/
 private def prodRel (scanIt' scanIt : @IterM (ScanM α m n β γ f) n γ) : Prop :=
-  (⟨scanIt'.internalState.inner⟩ : IterM m β).IsPlausibleSkipSuccessorOf
-    ⟨scanIt.internalState.inner⟩
+  (⟨scanIt'.internalState.inner⟩ : IterM m β).IsPlausibleSkipSuccessorOf ⟨scanIt.internalState.inner⟩
 
 private theorem acc_prodRel [Productive α m (β := β)]
-    (scanIt : @IterM (ScanM α m n β γ f) n γ)
-  : Acc prodRel scanIt
-  := by
-    generalize hgen : (⟨scanIt.internalState.inner⟩ : IterM m β) = innerIt
-    induction Productive.wf.apply innerIt generalizing scanIt with grind only [prodRel, Acc]
+    (scanIt : @IterM (ScanM α m n β γ f) n γ) :
+    Acc prodRel scanIt := by
+  generalize hgen : (⟨scanIt.internalState.inner⟩ : IterM m β) = innerIt
+  induction Productive.wf.apply innerIt generalizing scanIt with grind only [prodRel, Acc]
 
-private instance instProdRel [Monad m] [Monad n] [MonadLiftT m n] [Productive α m (β := β)] :
+private def instProdRel [Monad m] [Monad n] [MonadLiftT m n] [Productive α m (β := β)] :
     ProductivenessRelation (ScanM α m n β γ f) n where
   rel := prodRel
   wf := ⟨acc_prodRel⟩
@@ -178,18 +173,17 @@ private instance instProdRel [Monad m] [Monad n] [MonadLiftT m n] [Productive α
     intro _ _ hsucc
     cases hsucc <;> simp_all [prodRel, IterM.IsPlausibleSkipSuccessorOf]
 
-instance [Productive α m (β := β)] [Monad m] [Monad n] [MonadLiftT m n]
-    : Productive (ScanM α m n β γ f) n :=
+instance [Productive α m (β := β)] [Monad m] [Monad n] [MonadLiftT m n] :
+    Productive (ScanM α m n β γ f) n :=
   .of_productivenessRelation instProdRel
 
 end ScanM
-
 
 section Combinators
 variable {α β γ : Type w}
 
 section Monadic
-variable {m : Type w → Type w'} [Iterator α m β]
+variable {m : Type w → Type w'}
 
 /--
 If `it` is an iterator, then `it.scanM f init` is another iterator that folds a
@@ -219,9 +213,7 @@ it.scanM   init---a'-b'-c'-⊥
 For each value emitted by the base iterator `it`, this combinator calls `f`.
 -/
 @[inline, expose]
-def IterM.scanM {n : Type w → Type w''}
-    [Monad n] [MonadLiftT m n] (f : γ → β → n γ) (init : γ)
-    (it : IterM (α := α) m β) :=
+def IterM.scanM {n : Type w → Type w''} (f : γ → β → n γ) (init : γ) (it : IterM (α := α) m β) :=
   toIterM { inner := it.internalState, acc := init, emittedInit := false : ScanM α m n β γ f } n γ
 
 /--
@@ -257,12 +249,11 @@ def IterM.scan [Monad m]
 end Monadic
 
 @[inline, expose, inherit_doc IterM.scanM]
-def Iter.scanM {n : Type w → Type w''} [Iterator α Id β] [Monad n] [MonadLiftT Id n]
-    (f : γ → β → n γ) (init : γ) (it : Iter (α := α) β) :=
+def Iter.scanM {n : Type w → Type w''} (f : γ → β → n γ) (init : γ) (it : Iter (α := α) β) :=
   IterM.scanM f init it.toIterM
 
 @[inline, expose, inherit_doc IterM.scan]
-def Iter.scan [Iterator α Id β] (f : γ → β → γ) (init : γ) (it : Iter (α := α) β) :=
+def Iter.scan (f : γ → β → γ) (init : γ) (it : Iter (α := α) β) :=
   Iter.scanM (n := Id) (pure <| f · ·) init it |>.toIter
 
 end Combinators
